ulib/experimental/FStar.Reflection.Typing.fsti
@@ -28,10 +28,9 @@ module FStar.Reflection.Typing
   *)
 
 open FStar.List.Tot
-open FStar.Reflection
-module R = FStar.Reflection
-module T = FStar.Tactics
-module FTB = FStar.Tactics.Builtins
+open FStar.Reflection.V2
+module R = FStar.Reflection.V2
+module T = FStar.Tactics.V2
 
 val inspect_pack (t:R.term_view)
   : Lemma (ensures R.(inspect_ln (pack_ln t) == t))
@@ -42,6 +41,14 @@ val pack_inspect (t:R.term)
           (ensures R.(pack_ln (inspect_ln t) == t))
           [SMTPat R.(pack_ln (inspect_ln t))]
   
+val inspect_pack_namedv (t:R.namedv_view)
+  : Lemma (ensures R.(inspect_namedv (pack_namedv t) == t))
+          [SMTPat R.(inspect_namedv (pack_namedv t))]
+
+val pack_inspect_namedv (t:R.namedv)
+  : Lemma (ensures R.(pack_namedv (inspect_namedv t) == t))
+          [SMTPat R.(pack_namedv (inspect_namedv t))]
+
 val inspect_pack_bv (t:R.bv_view)
   : Lemma (ensures R.(inspect_bv (pack_bv t) == t))
           [SMTPat R.(inspect_bv (pack_bv t))]
@@ -58,30 +65,30 @@ val pack_inspect_binder (t:R.binder)
    : Lemma (ensures (R.pack_binder (R.inspect_binder t) == t))
            [SMTPat (R.pack_binder (R.inspect_binder t))]
   
+val inspect_pack_comp (t:R.comp_view)
+  : Lemma (ensures (R.inspect_comp (R.pack_comp t) == t))
+          [SMTPat (R.inspect_comp (R.pack_comp t))]
+
 val pack_inspect_comp (t:R.comp)
   : Lemma (ensures (R.pack_comp (R.inspect_comp t) == t))
           [SMTPat (R.pack_comp (R.inspect_comp t))]
   
-val inspect_pack_comp (t:R.comp_view)
-  : Lemma (ensures (R.inspect_comp (R.pack_comp t) == t))
-          [SMTPat (R.inspect_comp (R.pack_comp t))]
+val inspect_pack_fv (nm:R.name)
+  : Lemma (ensures R.inspect_fv (R.pack_fv nm) == nm)
+          [SMTPat (R.inspect_fv (R.pack_fv nm))]
 
 val pack_inspect_fv (fv:R.fv)
   : Lemma (ensures R.pack_fv (R.inspect_fv fv) == fv)
           [SMTPat (R.pack_fv (R.inspect_fv fv))]
 
-val inspect_pack_fv (nm:R.name)
-  : Lemma (ensures R.inspect_fv (R.pack_fv nm) == nm)
-          [SMTPat (R.inspect_fv (R.pack_fv nm))]
+val inspect_pack_universe (u:R.universe_view)
+  : Lemma (ensures R.inspect_universe (R.pack_universe u) == u)
+          [SMTPat (R.inspect_universe (R.pack_universe u))]
 
 val pack_inspect_universe (u:R.universe)
   : Lemma (requires ~(Uv_Unk? (inspect_universe u)))
           (ensures R.pack_universe (R.inspect_universe u) == u)
           [SMTPat (R.pack_universe (R.inspect_universe u))]
-
-val inspect_pack_universe (u:R.universe_view)
-  : Lemma (ensures R.inspect_universe (R.pack_universe u) == u)
-          [SMTPat (R.inspect_universe (R.pack_universe u))]
 
 val lookup_bvar (e:env) (x:int) : option term
 
@@ -93,16 +100,32 @@ let pp_name_t = FStar.Sealed.Inhabited.sealed "x"
 let pp_name_default : pp_name_t = FStar.Sealed.Inhabited.seal "x"
 let seal_pp_name x : pp_name_t = FStar.Sealed.Inhabited.seal x
 
-let mk_binder (pp_name:pp_name_t) (x:var) (ty:term) (q:aqualv)
+let tun = pack_ln Tv_Unknown
+
+let sort_t = FStar.Sealed.Inhabited.sealed tun
+let sort_default : sort_t = FStar.Sealed.Inhabited.seal tun
+let seal_sort x : sort_t = FStar.Sealed.Inhabited.seal x
+
+let mk_binder (pp_name:pp_name_t) (ty:term) (q:aqualv) : binder
   = pack_binder
-      { binder_bv=pack_bv ({bv_ppname=pp_name;
-                            bv_index=x});
-        binder_qual=q;
-        binder_attrs=[];
-        binder_sort=ty}
+      { ppname = pp_name;
+        qual   = q;
+        attrs  = [];
+        sort   = ty}
+
+let mk_simple_binder (pp_name:pp_name_t) (ty:term) : simple_binder
+  = pack_binder
+      { ppname = pp_name;
+        qual   = Q_Explicit;
+        attrs  = [];
+        sort   = ty}
 
 let extend_env (e:env) (x:var) (ty:term) : env =
-  R.push_binder e (mk_binder (seal_pp_name "x") x ty Q_Explicit)
+  R.push_binding e ({
+    ppname = seal_pp_name "x";
+    uniq   = x;
+    sort   = ty;
+  })
   
 val lookup_bvar_extend_env (g:env) (x y:var) (ty:term)
   : Lemma 
@@ -117,18 +140,19 @@ val lookup_fvar_extend_env (g:env) (x:fv) (us:universes) (y:var) (ty:term)
     (ensures lookup_fvar_uinst (extend_env g y ty) x us == lookup_fvar_uinst g x us)
     [SMTPat (lookup_fvar_uinst (extend_env g y ty) x us)]
 
-let as_binder (x:var) (ty:term) =
-  mk_binder (seal_pp_name "x") x ty Q_Explicit
-
 let bv_index (x:bv)
   : var
-  = (inspect_bv x).bv_index
+  = (inspect_bv x).index
+
+let namedv_uniq (x:namedv)
+  : var
+  = (inspect_namedv x).uniq
 
 let binder_sort (b:binder) =
-  (inspect_binder b).binder_sort
+  (inspect_binder b).sort
 
 let binder_qual (b:binder) =
-  let { binder_qual = q } = inspect_binder b in q
+  let { qual = q } = inspect_binder b in q
 
 noeq
 type open_or_close =
@@ -136,20 +160,42 @@ type open_or_close =
   | CloseVar of var
   | Rename   : var -> var -> open_or_close
 
-let tun = pack_ln Tv_Unknown
-
-let make_bv (n:nat) = {
-  bv_ppname = pp_name_default;
-  bv_index = n;
+let make_bv (n:nat) : bv_view = {
+  index  = n;
+  ppname = pp_name_default;
+  sort   = sort_default;
 }
-let make_bv_with_name (s:pp_name_t) (n:nat) = {
-  bv_ppname = s;
-  bv_index = n;
-}
-let var_as_bv (v:nat) = pack_bv (make_bv v)
-let var_as_term (v:var) = pack_ln (Tv_Var (var_as_bv v))
 
-let binder_of_t_q t q = mk_binder pp_name_default 0 t q
+let make_bv_with_name (s:pp_name_t) (n:nat) : bv_view = {
+  ppname = s;
+  index  = n;
+  sort   = sort_default;
+}
+
+let make_namedv (n:nat) : namedv_view = {
+  ppname = pp_name_default;
+  uniq   = n;
+  sort   = sort_default;
+}
+
+let make_namedv_with_name (s:pp_name_t) (n:nat) : namedv_view = {
+  ppname = s;
+  uniq   = n;
+  sort   = sort_default;
+}
+
+let var_as_bv (v:nat) : bv = pack_bv (make_bv v)
+
+let var_as_namedv (v:nat) : namedv =
+  pack_namedv {
+    uniq = v;
+    sort = sort_default;
+    ppname = pp_name_default;
+  }
+
+let var_as_term (v:var) = pack_ln (Tv_Var (var_as_namedv v))
+
+let binder_of_t_q t q = mk_binder pp_name_default t q
 let mk_abs ty qual t : R.term =  R.pack_ln (R.Tv_Abs (binder_of_t_q ty qual) t)
 let mk_total t = pack_comp (C_Total t)
 let mk_ghost t = pack_comp (C_GTotal t)
@@ -158,14 +204,22 @@ let mk_arrow ty qual t : R.term =
 let mk_ghost_arrow ty qual t : R.term =
   R.pack_ln (R.Tv_Arrow (binder_of_t_q ty qual) (mk_ghost t))
 let bound_var i : R.term = R.pack_ln (R.Tv_BVar (R.pack_bv (make_bv i)))
-let mk_let ppname (e1 t1 e2:R.term) =
-  R.pack_ln (R.Tv_Let false [] (R.pack_bv (make_bv_with_name ppname 0)) t1 e1 e2)
 
-let open_with_var (x:var) = OpenWith (pack_ln (Tv_Var (var_as_bv x)))
+let mk_let ppname (e1 t1 e2:R.term) =
+  let b : simple_binder = pack_binder ({
+    ppname = ppname;
+    sort   = t1;
+    qual   = Q_Explicit;
+    attrs  = [];
+  })
+  in
+  R.pack_ln (R.Tv_Let false [] b e1 e2)
+
+let open_with_var (x:var) = OpenWith (pack_ln (Tv_Var (var_as_namedv x)))
   
 let maybe_index_of_term (x:term) =
   match inspect_ln x with
-  | Tv_Var bv -> Some (bv_index bv)
+  | Tv_Var v -> Some ((inspect_namedv v).uniq)
   | _ -> None
   
 val open_or_close_ctx_uvar_and_subst (c:ctx_uvar_and_subst) (v:open_or_close) (i:nat) 
@@ -188,8 +242,8 @@ and binder_offset_pattern (p:pattern)
 
     | Pat_Var _ _ -> 1
 
-    | Pat_Cons fv us pats -> 
-      binder_offset_patterns pats
+    | Pat_Cons head univs subpats ->
+      binder_offset_patterns subpats
 
 let rec open_or_close_term' (t:term) (v:open_or_close) (i:nat)
   : Tot term (decreases t)
@@ -204,12 +258,12 @@ let rec open_or_close_term' (t:term) (v:open_or_close) (i:nat)
       (match v with
        | OpenWith _ -> t
        | CloseVar y ->
-         if bv_index x = y 
-         then pack_ln (Tv_BVar (pack_bv { inspect_bv x with bv_index = i }))
+         if namedv_uniq x = y 
+         then pack_ln (Tv_BVar (pack_bv { index = i; sort = (inspect_namedv x).sort; ppname = (inspect_namedv x).ppname }))
          else t
        | Rename y z ->
-         if bv_index x = y
-         then pack_ln (Tv_Var (pack_bv { inspect_bv x with bv_index = z }))
+         if namedv_uniq x = y
+         then pack_ln (Tv_Var (pack_namedv { inspect_namedv x with uniq = z }))
          else t)
 
     | Tv_BVar j -> 
@@ -223,7 +277,7 @@ let rec open_or_close_term' (t:term) (v:open_or_close) (i:nat)
            | None -> v
            | Some k ->
              //if we're substituting a name j for a name k, retain the pp_name of j
-             pack_ln (Tv_Var (pack_bv { inspect_bv j with bv_index = k }))
+             pack_ln (Tv_Var (pack_namedv { uniq = k; ppname = (inspect_bv j).ppname; sort = (inspect_bv j).sort }))
          )
          else t
       )
@@ -240,18 +294,20 @@ let rec open_or_close_term' (t:term) (v:open_or_close) (i:nat)
       let b' = open_or_close_binder' b v i in
       pack_ln (Tv_Arrow b' (open_or_close_comp' c v (i + 1)))      
 
-    | Tv_Refine bv sort f ->
-      pack_ln (Tv_Refine bv (open_or_close_term' sort v i)
-                            (open_or_close_term' f v (i + 1)))
+    | Tv_Refine b f ->
+      let b = open_or_close_binder' b v i in
+      assume (binder_is_simple b);
+      pack_ln (Tv_Refine b (open_or_close_term' f v (i + 1)))
 
     | Tv_Uvar j c ->
       pack_ln (Tv_Uvar j (open_or_close_ctx_uvar_and_subst c v i))
       
-    | Tv_Let recf attrs bv ty def body ->
+    | Tv_Let recf attrs b def body ->
+      let b = open_or_close_binder' b v i in
+      assume (binder_is_simple b);
       pack_ln (Tv_Let recf 
                       (open_or_close_terms' attrs v i)
-                      bv
-                      (open_or_close_term' ty v i)
+                      b
                       (if recf 
                        then open_or_close_term' def v (i + 1)
                        else open_or_close_term' def v i)
@@ -283,10 +339,11 @@ let rec open_or_close_term' (t:term) (v:open_or_close) (i:nat)
 and open_or_close_binder' (b:binder) (v:open_or_close) (i:nat)
   : Tot binder (decreases b)
   = let bndr  = inspect_binder b in
-    pack_binder {binder_bv=bndr.binder_bv;
-                 binder_qual=bndr.binder_qual;
-                 binder_attrs=open_or_close_terms' bndr.binder_attrs v i;
-                 binder_sort=open_or_close_term' bndr.binder_sort v i}
+    pack_binder { ppname = bndr.ppname;
+                  qual = bndr.qual;
+                  attrs = open_or_close_terms' bndr.attrs v i;
+                  sort = open_or_close_term' bndr.sort v i;
+                }
 
 and open_or_close_comp' (c:comp) (v:open_or_close) (i:nat)
   : Tot comp (decreases c)
@@ -337,12 +394,12 @@ and open_or_close_pattern' (p:pattern) (v:open_or_close) (i:nat)
   = match p with
     | Pat_Constant _ -> p
 
-    | Pat_Cons fv us pats -> 
-      let pats = open_or_close_patterns' pats v i in
-      Pat_Cons fv us pats
+    | Pat_Cons head univs subpats ->
+      let subpats = open_or_close_patterns' subpats v i in
+      Pat_Cons head univs subpats
 
-    | Pat_Var bv st ->
-      Pat_Var bv st
+    | Pat_Var bv s ->
+      Pat_Var bv s
 
     | Pat_Dot_Term topt ->
       Pat_Dot_Term (match topt with
@@ -404,6 +461,10 @@ val bv_index_of_make_bv (n:nat)
   : Lemma (ensures bv_index (pack_bv (make_bv n)) == n)
           [SMTPat (bv_index (pack_bv (make_bv n)))]
 
+val namedv_uniq_of_make_namedv (n:nat)
+  : Lemma (ensures namedv_uniq (pack_namedv (make_namedv n)) == n)
+          [SMTPat (namedv_uniq (pack_namedv (make_namedv n)))]
+
 let constant_as_term (v:vconst) = pack_ln (Tv_Const v)
 let unit_exp = constant_as_term C_Unit
 let unit_fv = pack_fv unit_lid
@@ -433,7 +494,7 @@ let eq2 (u:universe) (t v0 v1:term)
 
 let b2t_lid : R.name = ["Prims"; "b2t"]
 let b2t_fv : R.fv = R.pack_fv b2t_lid
-let b2t_ty : R.term = R.(pack_ln (Tv_Arrow (as_binder 0 bool_ty) (mk_total (tm_type u_zero))))
+let b2t_ty : R.term = R.pack_ln (R.Tv_Arrow (mk_binder (seal "x") bool_ty Q_Explicit) (mk_total (tm_type u_zero)))
 
 
 ////////////////////////////////////////////////////////////////////////////////
@@ -454,7 +515,7 @@ let rec freevars (e:term)
     | Tv_Unsupp
     | Tv_BVar _ -> Set.empty
 
-    | Tv_Var x -> Set.singleton (bv_index x)
+    | Tv_Var x -> Set.singleton (namedv_uniq x)
        
     | Tv_App e1 (e2, _) ->
       Set.union (freevars e1) (freevars e2)
@@ -465,13 +526,13 @@ let rec freevars (e:term)
     | Tv_Arrow b c ->
       Set.union (freevars_binder b) (freevars_comp c)
 
-    | Tv_Refine bv sort f ->
-       freevars sort `Set.union`
+    | Tv_Refine b f ->
+       freevars (binder_sort b) `Set.union`
        freevars f
       
-    | Tv_Let recf attrs bv ty def body ->
+    | Tv_Let recf attrs b def body ->
       freevars_terms attrs `Set.union`
-      freevars ty `Set.union`
+      freevars (binder_sort b) `Set.union`
       freevars def `Set.union`
       freevars body
 
@@ -532,9 +593,8 @@ and freevars_terms (ts:list term)
 and freevars_binder (b:binder)
   : Tot (Set.set var) (decreases b)
   = let bndr  = inspect_binder b in
-    freevars bndr.binder_sort `Set.union`
-    freevars_terms bndr.binder_attrs 
-    
+    freevars bndr.sort `Set.union`
+    freevars_terms bndr.attrs 
 
 and freevars_pattern (p:pattern) 
   : Tot (Set.set var) (decreases p)
@@ -542,10 +602,10 @@ and freevars_pattern (p:pattern)
     | Pat_Constant _ ->
       Set.empty
 
-    | Pat_Cons fv us pats -> 
-      freevars_patterns pats
+    | Pat_Cons head univs subpats ->
+      freevars_patterns subpats
       
-    | Pat_Var bv _ -> Set.empty
+    | Pat_Var bv s -> Set.empty
 
     | Pat_Dot_Term topt ->
       freevars_opt topt freevars
@@ -603,16 +663,16 @@ let rec ln' (e:term) (n:int)
       ln'_binder b n &&
       ln'_comp c (n + 1)
 
-    | Tv_Refine bv sort f ->
-      ln' sort n &&
+    | Tv_Refine b f ->
+      ln'_binder b n &&
       ln' f (n + 1)
 
     | Tv_Uvar _ _ ->
       false
       
-    | Tv_Let recf attrs bv ty def body ->
+    | Tv_Let recf attrs b def body ->
       ln'_terms attrs n &&
-      ln' ty n &&
+      ln'_binder b n &&
       (if recf then ln' def (n + 1) else ln' def n) &&
       ln' body (n + 1)
 
@@ -664,8 +724,8 @@ and ln'_args (ts:list argv) (i:int)
 and ln'_binder (b:binder) (n:int)
   : Tot bool (decreases b)
   = let bndr  = inspect_binder b in
-    ln' bndr.binder_sort n &&
-    ln'_terms bndr.binder_attrs n
+    ln' bndr.sort n &&
+    ln'_terms bndr.attrs n
 
 and ln'_terms (ts:list term) (n:int)
   : Tot bool (decreases ts)
@@ -690,10 +750,10 @@ and ln'_pattern (p:pattern) (i:int)
   = match p with
     | Pat_Constant _ -> true
 
-    | Pat_Cons fv us pats -> 
-      ln'_patterns pats i
+    | Pat_Cons head univs subpats ->
+      ln'_patterns subpats i
       
-    | Pat_Var bv _ -> true
+    | Pat_Var bv s -> true
 
     | Pat_Dot_Term topt ->
       (match topt with
@@ -859,7 +919,7 @@ and univ_leq : universe -> universe -> Type0 =
     univ_leq u (u_max u v)
 
 let mk_if (scrutinee then_ else_:R.term) : R.term =
-  pack_ln (Tv_Match scrutinee None [(Pat_Constant C_True, then_); 
+  pack_ln (Tv_Match scrutinee None [(Pat_Constant C_True, then_);
                                     (Pat_Constant C_False, else_)])
 
 
@@ -946,13 +1006,13 @@ type typing : env -> term -> comp_typ -> Type0 =
     g:env ->
     e:term ->
     c:comp_typ ->
-    squash (FTB.typing_token g e c) ->
+    squash (T.typing_token g e c) ->
     typing g e c
 
   | T_Var : 
      g:env ->
-     x:bv { Some? (lookup_bvar g (bv_index x)) } ->
-     typing g (pack_ln (Tv_Var x)) (T.E_Total, Some?.v (lookup_bvar g (bv_index x)))
+     x:namedv { Some? (lookup_bvar g (namedv_uniq x)) } ->
+     typing g (pack_ln (Tv_Var x)) (T.E_Total, Some?.v (lookup_bvar g (namedv_uniq x)))
 
   | T_FVar :
      g:env ->
@@ -984,9 +1044,9 @@ type typing : env -> term -> comp_typ -> Type0 =
      ty_eff:T.tot_or_ghost ->
      typing g ty (ty_eff, tm_type u) ->
      typing (extend_env g x ty) (open_term body x) body_c ->
-     typing g (pack_ln (Tv_Abs (mk_binder pp_name 0 ty q) body))
+     typing g (pack_ln (Tv_Abs (mk_binder pp_name ty q) body))
               (T.E_Total,
-               pack_ln (Tv_Arrow (mk_binder pp_name 0 ty q)
+               pack_ln (Tv_Arrow (mk_binder pp_name ty q)
                                  (mk_comp (close_comp_typ body_c x))))
 
   | T_App :
@@ -1028,7 +1088,7 @@ type typing : env -> term -> comp_typ -> Type0 =
      t2_eff:T.tot_or_ghost ->
      typing g t1 (t1_eff, tm_type u1) ->
      typing (extend_env g x t1) (open_term t2 x) (t2_eff, tm_type u2) ->
-     typing g (pack_ln (Tv_Arrow (mk_binder pp_name 0 t1 q) (mk_comp (eff, t2))))
+     typing g (pack_ln (Tv_Arrow (mk_binder pp_name t1 q) (mk_comp (eff, t2))))
               (T.E_Total, tm_type (u_max u1 u2))
 
   | T_Refine:
@@ -1042,7 +1102,7 @@ type typing : env -> term -> comp_typ -> Type0 =
      e_eff:T.tot_or_ghost ->
      typing g t (t_eff, tm_type u1) ->
      typing (extend_env g x t) (open_term e x) (e_eff, tm_type u2) ->
-     typing g (pack_ln (Tv_Refine (pack_bv (make_bv 0)) t e)) (T.E_Total, tm_type u1)
+     typing g (pack_ln (Tv_Refine (mk_simple_binder pp_name_default t) e)) (T.E_Total, tm_type u1)
 
   | T_PropIrrelevance:
      g:env -> 
@@ -1102,7 +1162,7 @@ and related : env -> term -> relation -> term -> Type0 =
     g:env ->
     t0:term ->
     t1:term ->
-    squash (FTB.subtyping_token g t0 t1) ->
+    squash (T.subtyping_token g t0 t1) ->
     related g t0 R_Sub t1
 
   | Rel_arrow:
@@ -1183,7 +1243,7 @@ and equiv : env -> term -> term -> Type0 =
     g:env ->
     t0:term ->
     t1:term ->
-    squash (FTB.equiv_token g t0 t1) ->
+    squash (T.equiv_token g t0 t1) ->
     equiv g t0 t1
 
   | EQ_Ctxt:
@@ -1241,10 +1301,10 @@ val subtyping_token_renaming (g:env)
                              (y:var { None? (lookup_bvar (extend_env_l g (bs1@bs0)) y) })
                              (t:term)
                              (t0 t1:term)
-                             (d:FTB.subtyping_token (extend_env_l g (bs1@(x,t)::bs0)) t0 t1)
-  : FTB.subtyping_token (extend_env_l g (rename_bindings bs1 x y@(y,t)::bs0))
-                        (rename t0 x y)
-                        (rename t1 x y)
+                             (d:T.subtyping_token (extend_env_l g (bs1@(x,t)::bs0)) t0 t1)
+  : T.subtyping_token (extend_env_l g (rename_bindings bs1 x y@(y,t)::bs0))
+                      (rename t0 x y)
+                      (rename t1 x y)
 
 val subtyping_token_weakening (g:env)
                               (bs0:bindings)
@@ -1252,8 +1312,8 @@ val subtyping_token_weakening (g:env)
                               (x:var { None? (lookup_bvar (extend_env_l g (bs1@bs0)) x) })
                               (t:term)
                               (t0 t1:term)
-                              (d:FTB.subtyping_token (extend_env_l g (bs1@bs0)) t0 t1)
-  : FTB.subtyping_token (extend_env_l g (bs1@(x,t)::bs0)) t0 t1
+                              (d:T.subtyping_token (extend_env_l g (bs1@bs0)) t0 t1)
+  : T.subtyping_token (extend_env_l g (bs1@(x,t)::bs0)) t0 t1
 
 let simplify_umax (#g:R.env) (#t:R.term) (#u:R.universe)
                   (d:typing g t (T.E_Total, tm_type (u_max u u)))
