ulib/FStar.Tactics.Print.fst
@@ -1,9 +1,13 @@
 module FStar.Tactics.Print
 
-open FStar.Reflection
+open FStar.Reflection.V2
 open FStar.Tactics.Effect
-open FStar.Tactics.Builtins
-open FStar.Tactics.Derived
+open FStar.Tactics.V2.Builtins
+open FStar.Tactics.V2.Derived
+open FStar.Tactics.NamedView
+
+let namedv_to_string (x:namedv) : Tac string=
+  unseal x.ppname ^ "#" ^ string_of_int x.uniq
 
 private
 let paren (s:string) : string = "(" ^ s ^ ")"
@@ -35,7 +39,7 @@ let universes_to_ast_string (us:universes) : Tac string =
 
 let rec term_to_ast_string (t:term) : Tac string =
   match inspect t with
-  | Tv_Var bv -> "Tv_Var " ^ bv_to_string bv
+  | Tv_Var bv -> "Tv_Var " ^ namedv_to_string bv
   | Tv_BVar bv -> "Tv_BVar " ^ bv_to_string bv
   | Tv_FVar fv -> "Tv_FVar " ^ fv_to_string fv
   | Tv_UInst fv us ->
@@ -44,12 +48,12 @@ let rec term_to_ast_string (t:term) : Tac string =
   | Tv_Abs x e -> "Tv_Abs " ^ paren (binder_to_string x ^ ", " ^ term_to_ast_string e)
   | Tv_Arrow x c -> "Tv_Arrow " ^ paren (binder_to_string x ^ ", " ^ comp_to_ast_string c)
   | Tv_Type u -> "Type" ^ paren (universe_to_ast_string u)
-  | Tv_Refine x sort e -> "Tv_Refine " ^ paren (bv_to_string x ^ ", " ^ term_to_ast_string sort ^", " ^ term_to_ast_string e)
+  | Tv_Refine x e -> "Tv_Refine " ^ paren (binder_to_string x ^ ", " ^ term_to_ast_string e)
   | Tv_Const c -> const_to_ast_string c
   | Tv_Uvar i _ -> "Tv_Uvar " ^ string_of_int i
-  | Tv_Let recf _ x _ e1 e2 ->
+  | Tv_Let recf _ x e1 e2 ->
            "Tv_Let " ^ paren (string_of_bool recf ^ ", " ^
-                              bv_to_string x ^ ", " ^
+                              binder_to_string x ^ ", " ^
                               term_to_ast_string e1 ^ ", " ^
                               term_to_ast_string e2)
   | Tv_Match e ret_opt brs ->
